Auto/Lib/HList.lean
@@ -10,6 +10,14 @@ def HList.getD {β : α → Sort _} {ty : α} (default : β ty) :
   | .(_), .cons a _,  0       => a
   | .(_), .cons _ as, .succ n => HList.getD default as n
 
+theorem HList.getD_heq
+  {β₁ : α₁ → Sort _} {ty₁ : α₁} {default₁ : β₁ ty₁} {tys₁ : List α₁} {hl₁ : HList β₁ tys₁} {n₁ : Nat}
+  {β₂ : α₂ → Sort _} {ty₂ : α₂} {default₂ : β₂ ty₂} {tys₂ : List α₂} {hl₂ : HList β₂ tys₂} {n₂ : Nat}
+  (hβ : HEq β₁ β₂) (hty : HEq ty₁ ty₂) (hdefault : HEq default₁ default₂)
+  (htys : HEq tys₁ tys₂) (hhl : HEq hl₁ hl₂) (hn : n₁ = n₂) :
+  HEq (HList.getD default₁ hl₁ n₁) (HList.getD default₂ hl₂ n₂) := by
+  cases hty; cases hβ; cases hdefault; cases htys; cases hhl; cases hn; apply HEq.rfl
+
 def HList.ofMapTy {γ : β → Sort _} (f : α → β) :
   {tys : List α} → HList γ (List.map f tys) → HList (γ ∘ f) tys
   | .nil,      .nil       => .nil
@@ -28,5 +36,15 @@ def HList.map {β : α → Sort _} {γ : α → Sort _} (f : ∀ (a : α), β a 
   {tys : List α} → (xs : HList β tys) → HList γ tys
   | .nil,      .nil       => .nil
   | .cons _ _, .cons x xs => .cons (f _ x) (map f xs)
+
+def HList.reverseAux : {as : _} → (xs : HList β as) → (ys : HList β bs) → HList β (List.reverseAux as bs)
+  | .nil,       .nil,       r => r
+  | .cons _ as, .cons x xs, r => reverseAux (as:=as) xs (.cons x r)
+
+def HList.reverse (xs : HList β as) : HList β (List.reverse as) := HList.reverseAux xs .nil
+
+def HList.append : (xs : HList β as) → (ys : HList β bs) → HList β (as.append bs)
+  | .nil,       ys => ys
+  | .cons x xs, ys => .cons x (append xs ys)
 
 end Auto
